src/HOL/IMP/Procs.thy
@@ -4,15 +4,17 @@ theory Procs imports BExp begin
 
 subsection "Procedures and Local Variables"
 
+type_synonym pname = string
+
 datatype
   com = SKIP 
-      | Assign name aexp         ("_ ::= _" [1000, 61] 61)
+      | Assign vname aexp        ("_ ::= _" [1000, 61] 61)
       | Semi   com  com          ("_;/ _"  [60, 61] 60)
       | If     bexp com com     ("(IF _/ THEN _/ ELSE _)"  [0, 0, 61] 61)
       | While  bexp com         ("(WHILE _/ DO _)"  [0, 61] 61)
-      | Var    name com         ("(1{VAR _;;/ _})")
-      | Proc   name com com     ("(1{PROC _ = _;;/ _})")
-      | CALL   name
+      | Var    vname com        ("(1{VAR _;;/ _})")
+      | Proc   pname com com    ("(1{PROC _ = _;;/ _})")
+      | CALL   pname
 
 definition "test_com =
 {VAR ''x'';;
